Connected multiplier and divider to an impl. (Now working on the correctness proof)

Puar/MulDiv.v
@@ -1,259 +1,10 @@
 Require Import Kami.
 Require Import Lib.Indexer Lib.Struct Lib.FMap Lib.Reflection.
 Require Import Kami.Tactics Kami.SemFacts.
-Require Import Puar.Useful Puar.Processor FunctionalExtensionality.
-
-(* Below implements a radix-4 Booth Multiplier. *)
-Section Multiplier64.
-  (* NOTE: hard to declare [LogNumPhases] and [NumBitsPerPhase] as variables,
-   * since truncation and extension require certain equation w.r.t. bit-lengths.
-   *)
-  (* Variable MultLogNumPhases MultNumBitsPerPhase: nat. *)
-  Definition MultLogNumPhases := 3.
-  Definition MultNumBitsPerPhase := 8.
-
-  Local Definition MultNumPhases := wordToNat (wones MultLogNumPhases) + 1.
-  Local Definition MultNumBits := MultNumPhases * MultNumBitsPerPhase.
-  Local Definition MultBits := 2 * MultNumBits + 2.
-
-  Definition MultInStr := STRUCT { "multiplicand" :: Bit MultNumBits;
-                                   "multiplier" :: Bit MultNumBits }.
-  Definition MultOutStr := STRUCT { "high" :: Bit MultNumBits;
-                                    "low" :: Bit MultNumBits }.
-
-  Definition multRegister := MethodSig "multRegister"(Struct MultInStr): Void.
-  Definition multGetResult := MethodSig "multGetResult"(Void): Struct MultOutStr.
-
-  Definition boothStep' {ty}
-             (m_pos m_neg: fullType ty (SyntaxKind (Bit MultBits)))
-             (p: Expr ty (SyntaxKind (Bit MultBits)))
-             (pr: Expr ty (SyntaxKind (Bit 3))) :=
-    (IF (pr == $$(WO~0~0~0)) then p
-     else IF (pr == $$(WO~0~0~1)) then p + #m_pos
-     else IF (pr == $$(WO~0~1~0)) then p + #m_pos
-     else IF (pr == $$(WO~0~1~1)) then p + (#m_pos << $$(WO~1))
-     else IF (pr == $$(WO~1~0~0)) then p + (#m_pos << $$(WO~1))
-     else IF (pr == $$(WO~1~0~1)) then p + #m_neg
-     else IF (pr == $$(WO~1~1~0)) then p + #m_neg
-     else p)%kami_expr.
-
-  Definition boothStep {ty}
-             (m_pos m_neg: fullType ty (SyntaxKind (Bit MultBits)))
-             (p: Expr ty (SyntaxKind (Bit ((MultBits - 3) + 3))))
-    : Expr ty (SyntaxKind (Bit MultBits)) :=
-    (boothStep' m_pos m_neg p (UniBit (Trunc 3 _) p) >> $$(WO~1~0))%kami_expr.
-
-  Fixpoint boothSteps (cnt: nat)
-           {ty} (m_pos m_neg: fullType ty (SyntaxKind (Bit MultBits)))
-           (p: fullType ty (SyntaxKind (Bit ((MultBits - 3) + 3))))
-           (cont: fullType ty (SyntaxKind (Bit ((MultBits - 3) + 3))) ->
-                  ActionT ty Void)
-    : ActionT ty Void :=
-    match cnt with
-    | O => (cont p)%kami_action
-    | S n => (LET np <- boothStep m_pos m_neg #p;
-              boothSteps n m_pos m_neg np cont)%kami_action
-    end.
-
-  Definition boothMultiplierImpl :=
-    MODULE {
-      Register "m_pos" : Bit MultBits <- Default
-      with Register "m_neg" : Bit MultBits <- Default
-      with Register "p" : Bit MultBits <- Default
-      with Register "cnt" : Bit (S MultLogNumPhases) <- Default
-
-      with Method "multRegister"(src: Struct MultInStr): Void :=
-        LET m : Bit (pred MultNumBits + 1) <- #src!MultInStr@."multiplicand";
-        LET m_msb <- UniBit (TruncLsb _ 1) #m;
-        LET m_neg <- (UniBit (Inv _) #m) + $1;
-        LET m_neg_msb <- UniBit (TruncLsb _ 1) #m_neg;
-        
-        Write "m_pos" : Bit MultBits <-
-          BinBit (Concat _ (S MultNumBits)) (BinBit (Concat _ _) #m_msb #m) $0;
-        Write "m_neg" : Bit MultBits <-
-          BinBit (Concat _ (S MultNumBits)) (BinBit (Concat _ _) #m_neg_msb #m_neg) $0;
-        
-        LET r <- #src!MultInStr@."multiplier";
-        Write "p" : Bit MultBits <-
-          BinBit (Concat (S MultNumBits) _) $0 (BinBit (Concat _ 1) #r $0);
-
-        Write "cnt" : Bit (S MultLogNumPhases) <- $(MultNumPhases);
-        Retv
-
-      with Method "multGetResult"(): Struct MultOutStr :=
-        Read cnt : Bit MultLogNumPhases <- "cnt";
-        Assert (#cnt == $0);
-
-        Read p : Bit MultBits <- "p";
-        LET high : Bit MultNumBits <- UniBit (ConstExtract (S MultNumBits) MultNumBits 1) #p;
-        LET low : Bit MultNumBits <- UniBit (ConstExtract 1 MultNumBits (S MultNumBits)) #p;
-
-        LET ret : Struct MultOutStr <- STRUCT { "high" ::= $$Default; "low" ::= #low };
-        Ret #ret
-            
-      with Rule "boothStep" :=
-        Read cnt : Bit MultLogNumPhases <- "cnt";
-        Assert (#cnt != $0);
-
-        Read m_pos : Bit MultBits <- "m_pos";
-        Read m_neg : Bit MultBits <- "m_neg";
-        Read p : Bit MultBits <- "p";
-
-        boothSteps
-          MultNumBitsPerPhase m_pos m_neg p
-          (fun np => Write "p" <- #np; Retv)
-    }.
-
-  Definition multiplierSpec :=
-    MODULE {
-      Register "p" : Bit (2 * MultNumBits) <- Default
-
-      with Method "multRegister"(src: Struct MultInStr): Void :=
-        LET m : Bit MultNumBits <- #src!MultInStr@."multiplicand";
-        LET m_ext : Bit (2 * MultNumBits) <- UniBit (SignExtendTrunc _ _) #m;
-        LET r : Bit MultNumBits <- #src!MultInStr@."multiplier";
-        LET r_ext : Bit (2 * MultNumBits) <- UniBit (SignExtendTrunc _ _) #m;
-
-        Write "p" <- #m_ext *s #r_ext;
-        Retv
-
-      with Method "multGetResult"(): Struct MultOutStr :=
-        Read p : Bit (MultNumBits + MultNumBits) <- "p";
-        LET high : Bit MultNumBits <- UniBit (TruncLsb _ _) #p;
-        LET low : Bit MultNumBits <- UniBit (Trunc _ _) #p;
-
-        LET ret : Struct MultOutStr <- STRUCT { "high" ::= #high; "low" ::= #low };
-        Ret #ret
-    }.
-
-End Multiplier64.
-
-(* Below implements non-restoring division for unsigned integers.
- * Operand signs are re-applied after the division.
- * NOTE: the rule for operand signs:
- * when "z = d * q + r", we have "sign(r) = sign(z)" and "|r| < |d|".
- *)
-Section Divider64.
-  Definition DivLogNumPhases := 3.
-  Definition DivNumBitsPerPhase := 8.
-
-  Local Definition DivNumPhases := wordToNat (wones DivLogNumPhases) + 1.
-  Local Definition DivNumBits := DivNumPhases * DivNumBitsPerPhase.
-  Local Definition DivBits := 2 * DivNumBits + 2.
-
-  Definition DivInStr := STRUCT { "dividend" :: Bit DivNumBits;
-                                  "divisor" :: Bit DivNumBits }.
-  Definition DivOutStr := STRUCT { "quotient" :: Bit DivNumBits;
-                                   "remainder" :: Bit DivNumBits }.
-
-  Definition divRegister := MethodSig "divRegister"(Struct DivInStr): Void.
-  Definition divGetResult := MethodSig "divGetResult"(Void): Struct DivOutStr.
-
-  (*! TODO: optimize this step !*)
-  Definition divStep {ty}
-             (pq: fullType ty (SyntaxKind (Bit (DivNumBits + S DivNumBits))))
-             (dr: fullType ty (SyntaxKind (Bit DivNumBits)))
-    : Expr ty (SyntaxKind (Bit (DivNumBits + S DivNumBits))) :=
-    ((* Step 1: shift *)
-      let pq_shift := BinBit (Sll ((DivNumBits + DivNumBits) + 1) _) #pq $$(natToWord 1 1) in
-      (* Step 2: add or subtract *)
-      let pq_shift_msb := UniBit (TruncLsb _ 1) pq_shift in
-      let pq_shift_p := (IF (pq_shift_msb == $0)
-                         then pq_shift - (BinBit (Concat _ (S DivNumBits)) #dr $0)
-                         else pq_shift + (BinBit (Concat _ (S DivNumBits)) #dr $0)) in
-      (* Step 3: set the quotient bit, which is LSB here *)
-      let pq_shift_p_msb := UniBit (TruncLsb _ 1) pq_shift_p in
-      IF (pq_shift_p_msb == $0)
-      then pq_shift_p + $1
-      else pq_shift_p
-    )%kami_expr.
-  
-  Fixpoint divSteps (cnt: nat)
-           {ty} (pq: fullType ty (SyntaxKind (Bit (DivNumBits + S DivNumBits))))
-           (dr: fullType ty (SyntaxKind (Bit DivNumBits)))
-           (cont: fullType ty (SyntaxKind (Bit (DivNumBits + S DivNumBits))) ->
-                  ActionT ty Void)
-    : ActionT ty Void :=
-    match cnt with
-    | O => (cont pq)%kami_action
-    | S n => (LET npq <- divStep pq dr;
-              divSteps n npq dr cont)%kami_action
-    end.
-
-  Definition nrDividerImpl :=
-    MODULE {
-      Register "pq" : Bit (DivNumBits + S DivNumBits) <- Default
-      with Register "dr" : Bit DivNumBits <- Default
-      with Register "cnt" : Bit (S DivLogNumPhases) <- Default
-
-      with Method "divRegister"(src: Struct DivInStr): Void :=
-        LET dividend : Bit DivNumBits <- #src!DivInStr@."dividend";
-        LET divisor : Bit DivNumBits <- #src!DivInStr@."divisor";
-
-        Write "pq" : Bit (DivNumBits + S DivNumBits) <- UniBit (ZeroExtendTrunc _ _) #dividend;
-        Write "dr" <- #divisor;
-        Write "cnt" : Bit (S DivLogNumPhases) <- $(DivNumPhases);
-        Retv
-
-      with Method "divGetResult"(): Struct DivOutStr :=
-        Read cnt : Bit DivLogNumPhases <- "cnt";
-        Assert (#cnt == $0);
-
-        Read pq : Bit (DivNumBits + S DivNumBits) <- "pq";
-        Read dr : Bit DivNumBits <- "dr";
-        
-        LET p : Bit (DivNumBits + 1) <- UniBit (TruncLsb _ _) #pq;
-        LET q : Bit DivNumBits <- UniBit (Trunc _ _) #pq;
-
-        LET p_msb <- UniBit (TruncLsb _ 1) #p;
-        LET p_ls : Bit DivNumBits <- UniBit (Trunc _ _) #p;
-        LET rem : Bit DivNumBits <- (IF (#p_msb == $0)
-                                     then #p_ls
-                                     else #p_ls + #dr);
-        
-        LET ret : Struct DivOutStr <- STRUCT { "quotient" ::= #q;
-                                               "remainder" ::= #rem
-                                             };
-        Ret #ret
-            
-      with Rule "divStep" :=
-        Read cnt : Bit DivLogNumPhases <- "cnt";
-        Assert (#cnt != $0);
-
-        Read pq : Bit (DivNumBits + S DivNumBits) <- "pq";
-        Read dr : Bit DivNumBits <- "dr";
-        
-        divSteps
-          DivNumBitsPerPhase pq dr
-          (fun npq => Write "pq" <- #npq; Retv)
-    }.
-
-  Definition dividerSpec :=
-    MODULE {
-      Register "quotient" : Bit DivNumBits <- Default
-      with Register "remainder" : Bit DivNumBits <- Default
-                         
-      with Method "DivRegister"(src: Struct DivInStr): Void :=
-        LET m : Bit DivNumBits <- #src!DivInStr@."dividend";
-        LET r : Bit DivNumBits <- #src!DivInStr@."divisor";
-
-        Write "quotient" <- #m /s #r;
-        Write "remainder" <- BinBit (Rem _ SignSS) #m #r;
-        Retv
-
-      with Method "DivGetResult"(): Struct DivOutStr :=
-        Read quotient : Bit DivNumBits <- "quotient";
-        Read remainder : Bit DivNumBits <- "remainder";
-
-        LET ret : Struct DivOutStr <- STRUCT { "quotient" ::= #quotient;
-                                               "remainder" ::= #remainder };
-        Ret #ret
-    }.
-  
-End Divider64.
+Require Import Puar.Useful Puar.Processor Puar.Multiplier Puar.Divider.
+Require Import FunctionalExtensionality.
 
 Section Processor.
-  Variable NumDataBytes: nat.
   Variables VAddr PAddr Inst Mode MemException ExecException: Kind.
 
   Variable isNotLongLat: forall ty, ty Inst -> Bool @ ty.
@@ -268,11 +19,11 @@ Section Processor.
   Definition MulDivSignUU : ConstT MulDivSign := WO~1~0.
   Variable getMulDivSign: forall ty, ty Inst -> MulDivSign @ ty.
 
-  Local Notation Exec := (Exec NumDataBytes VAddr ExecException).
-
   Section Spec.
+    Variable NumDataBytes: nat.
 
     Definition Data := Bit (8 * NumDataBytes).
+    Local Notation Exec := (Exec NumDataBytes VAddr ExecException).
 
     Definition execFnLongLatSpec ty (pc: ty VAddr)
                (inst: ty Inst) (val1 val2: ty Data)
@@ -313,23 +64,27 @@ Section Processor.
 
   End Spec.
 
-  Section Impl.
+  Section Impl64.
+    Definition NumDataBytes := 8.
+    Definition Data64 := Bit (8 * NumDataBytes).
 
+    Local Notation Exec := (Exec NumDataBytes VAddr ExecException).
     Local Notation regReadFirst := (regReadFirst NumDataBytes VAddr PAddr Inst Mode MemException).
     Local Notation regReadPop := (regReadPop NumDataBytes VAddr PAddr Inst Mode MemException).
     Local Notation RegReadT := (RegReadT NumDataBytes VAddr PAddr Inst Mode MemException).
     Local Notation execEnq := (execEnq NumDataBytes VAddr PAddr Inst Mode
                                        MemException ExecException).
 
-    Definition LongLatStr := STRUCT { "inst" :: Inst;
-                                      "src1" :: Data;
-                                      "src2" :: Data }.
-    Definition longLatRegister := MethodSig "longLatRegister"(Struct LongLatStr): Void.
-    Definition longLatGetResult := MethodSig "longLatGetResult"(Void): Struct Exec.
-
     Definition longLat :=
       MODULE {
-        Rule longLatStart :=
+        Register "llRegistered" : Bool <- false
+        with Register "llHasResult" : Bool <- false
+        with Register "llInst" : Inst <- Default
+        with Register "llSrc1" : Data64 <- Default
+        with Register "llSrc2" : Data64 <- Default
+        with Register "llRes" : Data64 <- Default
+                                        
+        with Rule longLatStart :=
           Call inp1 <- regReadFirst();
           LET instVal <- #inp1!RegReadT@.inst;
           Assert (! (isNotLongLat _ instVal));
@@ -347,7 +102,7 @@ Section Processor.
           Call writeLongLatCall($$ false);
           Retv
 
-        with Rule "longLatFinish_init" :=
+        with Rule "longLatWork" :=
           Call epochsMatchVal <- epochsMatchCall();
           Assert #epochsMatchVal;
           Call inp1 <- regReadFirst();
@@ -360,13 +115,104 @@ Section Processor.
           Assert #longLatVal;
           Call writeLongLatCall($$ false);
 
-          Call longLatRegister(STRUCT { "inst" ::= #instVal;
-                                        "src1" ::= #src1Val;
-                                        "src2" ::= #src2Val });
+          Read reg <- "llRegistered";
+          Assert !#reg;
+          Write "llRegistered" <- $$true;
+
+          Write "llInst" <- #instVal;
+          Write "llSrc1" <- #src1Val;
+          Write "llSrc2" <- #src2Val;
           Retv
 
+        with Rule "longLatMult" :=
+          Read reg <- "llRegistered";
+          Assert #reg;
+
+          Read inst : Inst <- "llInst";
+          Read src1 : Data64 <- "llSrc1";
+          Read src2 : Data64 <- "llSrc2";
+
+          Assert (isMul _ inst);
+
+          If (getMulDivSign _ inst == $$MulDivSignSS)
+          then
+            Call boothMultRegister(
+              STRUCT { "multiplicand" ::= UniBit (SignExtendTrunc _ _) #src1;
+                       "multiplier" ::= UniBit (SignExtendTrunc _ _) #src2 });
+            Retv
+          else
+            If (getMulDivSign _ inst == $$MulDivSignSU)
+            then
+              Call boothMultRegister(
+                STRUCT { "multiplicand" ::= UniBit (SignExtendTrunc _ _) #src1;
+                         "multiplier" ::= UniBit (ZeroExtendTrunc _ _) #src2 });
+              Retv
+            else
+              Call boothMultRegister(
+                STRUCT { "multiplicand" ::= UniBit (ZeroExtendTrunc _ _) #src1;
+                         "multiplier" ::= UniBit (ZeroExtendTrunc _ _) #src2 });
+              Retv;
+            Retv;
+          Retv
+
+        with Rule "longLatDiv" :=
+          Read reg <- "llRegistered";
+          Assert #reg;
+
+          Read inst : Inst <- "llInst";
+          Read src1 : Data64 <- "llSrc1";
+          Read src2 : Data64 <- "llSrc2";
+
+          Assert (isDiv _ inst || isRem _ inst);
+
+          If (getMulDivSign _ inst == $$MulDivSignSS)
+          then
+            Call nrDivRegister(
+              STRUCT { "dividend" ::= UniBit (ZeroExtendTrunc _ 64) (UniBit (Trunc 63 1) #src1);
+                       "divisor" ::= UniBit (ZeroExtendTrunc _ 64) (UniBit (Trunc 63 1) #src2) });
+            Retv
+          else
+            If (getMulDivSign _ inst == $$MulDivSignSU)
+            then
+              Call nrDivRegister(
+                STRUCT { "dividend" ::= UniBit (ZeroExtendTrunc _ 64) (UniBit (Trunc 63 1) #src1);
+                         "divisor" ::= #src2 });
+              Retv
+            else
+              Call nrDivRegister(STRUCT { "dividend" ::= #src1; "divisor" ::= #src2 });
+              Retv;
+            Retv;
+          Retv
+
+        with Rule "longLatMultFinish" :=
+          Read inst : Inst <- "llInst";
+          Assert (isMul _ inst);
+
+          Call mres <- boothMultGetResult();
+          (* TODO: write appropriate values to "llRes" *)
+
+          Write "llHasResult" <- $$true;
+          Retv
+
+        with Rule "longLatDivFinish" :=
+          Read inst : Inst <- "llInst";
+          Assert (isDiv _ inst || isRem _ inst);
+
+          Call dres <- nrDivGetResult();
+          (* TODO: write appropriate values to "llRes" *)
+
+          Write "llHasResult" <- $$true;
+          Retv
+            
         with Rule "longLatFinish_done" :=
-          Call execVal <- longLatGetResult();
+          Read hasResult <- "llHasResult";
+          Assert #hasResult;
+          Read res <- "llRes";
+          
+          LET execVal <- STRUCT { "data" ::= #res;
+                                  "memVAddr" ::= $$Default;
+                                  "exception" ::= $$Default;
+                                  "nextPc" ::= $$Default (* (pc + 4)? *) };
           Call inp1 <- regReadPop();
           Call execEnq(STRUCT { wbEpoch ::= #inp1!RegReadT@.wbEpoch;
                                 pc ::= #inp1!RegReadT@.pc;
@@ -374,12 +220,22 @@ Section Processor.
                                 inst ::= #inp1!RegReadT@.inst;
                                 exec ::= #execVal
                               });
+
+          Write "llRegistered" <- $$false;
+          Write "llHasResult" <- $$false;
           Retv
       }.
 
-    Definition longLatImpl := longLat. (* TODO: add handlers. *)
+    Definition longLatImpl :=
+      (longLat ++ boothMultiplierImpl ++ nrDividerImpl)%kami.
     
-  End Impl.
+  End Impl64.
 
+
+  Theorem longLat_refines:
+    longLatImpl <<== (longLatSpec NumDataBytes).
+  Proof.
+  Admitted.
+  
 End Processor.
 
