Puar/Divider.v
@@ -1,0 +1,135 @@
+Require Import Kami.
+Require Import Lib.Indexer Lib.Struct Lib.FMap Lib.Reflection.
+Require Import Kami.Tactics Kami.SemFacts.
+Require Import Puar.Useful FunctionalExtensionality.
+
+(* Below implements non-restoring division for _unsigned_ integers.
+ * Operands should be made unsigned first and the signs should be re-applied
+ * after the division.
+ * NOTE: the rule for operand signs:
+ * when "z = d * q + r", we have "sign(r) = sign(z)" and "|r| < |d|".
+ *)
+Section Divider64.
+  Definition DivLogNumPhases := 3.
+  Definition DivNumBitsPerPhase := 8.
+
+  Local Definition DivNumPhases := wordToNat (wones DivLogNumPhases) + 1.
+  Local Definition DivNumBits := DivNumPhases * DivNumBitsPerPhase.
+  Local Definition DivBits := 2 * DivNumBits + 2.
+
+  Definition DivInStr := STRUCT { "dividend" :: Bit DivNumBits;
+                                  "divisor" :: Bit DivNumBits }.
+  Definition DivOutStr := STRUCT { "quotient" :: Bit DivNumBits;
+                                   "remainder" :: Bit DivNumBits }.
+
+  Definition divRegister := MethodSig "divRegister"(Struct DivInStr): Void.
+  Definition divGetResult := MethodSig "divGetResult"(Void): Struct DivOutStr.
+
+  (*! TODO: optimize this step !*)
+  Definition divStep {ty}
+             (pq: fullType ty (SyntaxKind (Bit (DivNumBits + S DivNumBits))))
+             (dr: fullType ty (SyntaxKind (Bit DivNumBits)))
+    : Expr ty (SyntaxKind (Bit (DivNumBits + S DivNumBits))) :=
+    ((* Step 1: shift *)
+      let pq_shift := BinBit (Sll ((DivNumBits + DivNumBits) + 1) _) #pq $$(natToWord 1 1) in
+      (* Step 2: add or subtract *)
+      let pq_shift_msb := UniBit (TruncLsb _ 1) pq_shift in
+      let pq_shift_p := (IF (pq_shift_msb == $0)
+                         then pq_shift - (BinBit (Concat _ (S DivNumBits)) #dr $0)
+                         else pq_shift + (BinBit (Concat _ (S DivNumBits)) #dr $0)) in
+      (* Step 3: set the quotient bit, which is LSB here *)
+      let pq_shift_p_msb := UniBit (TruncLsb _ 1) pq_shift_p in
+      IF (pq_shift_p_msb == $0)
+      then pq_shift_p + $1
+      else pq_shift_p
+    )%kami_expr.
+  
+  Fixpoint divSteps (cnt: nat)
+           {ty} (pq: fullType ty (SyntaxKind (Bit (DivNumBits + S DivNumBits))))
+           (dr: fullType ty (SyntaxKind (Bit DivNumBits)))
+           (cont: fullType ty (SyntaxKind (Bit (DivNumBits + S DivNumBits))) ->
+                  ActionT ty Void)
+    : ActionT ty Void :=
+    match cnt with
+    | O => (cont pq)%kami_action
+    | S n => (LET npq <- divStep pq dr;
+              divSteps n npq dr cont)%kami_action
+    end.
+
+  Definition nrDivRegister :=
+    MethodSig "nrDivRegister"(Struct DivInStr): Void.
+  Definition nrDivGetResult :=
+    MethodSig "nrDivGetResult"(): Struct DivOutStr.
+
+  Definition nrDividerImpl :=
+    MODULE {
+      Register "pq" : Bit (DivNumBits + S DivNumBits) <- Default
+      with Register "dr" : Bit DivNumBits <- Default
+      with Register "cnt" : Bit (S DivLogNumPhases) <- Default
+
+      with Method "nrDivRegister"(src: Struct DivInStr): Void :=
+        LET dividend : Bit DivNumBits <- #src!DivInStr@."dividend";
+        LET divisor : Bit DivNumBits <- #src!DivInStr@."divisor";
+
+        Write "pq" : Bit (DivNumBits + S DivNumBits) <- UniBit (ZeroExtendTrunc _ _) #dividend;
+        Write "dr" <- #divisor;
+        Write "cnt" : Bit (S DivLogNumPhases) <- $(DivNumPhases);
+        Retv
+
+      with Method "nrDivGetResult"(): Struct DivOutStr :=
+        Read cnt : Bit DivLogNumPhases <- "cnt";
+        Assert (#cnt == $0);
+
+        Read pq : Bit (DivNumBits + S DivNumBits) <- "pq";
+        Read dr : Bit DivNumBits <- "dr";
+        
+        LET p : Bit (DivNumBits + 1) <- UniBit (TruncLsb _ _) #pq;
+        LET q : Bit DivNumBits <- UniBit (Trunc _ _) #pq;
+
+        LET p_msb <- UniBit (TruncLsb _ 1) #p;
+        LET p_ls : Bit DivNumBits <- UniBit (Trunc _ _) #p;
+        LET rem : Bit DivNumBits <- (IF (#p_msb == $0)
+                                     then #p_ls
+                                     else #p_ls + #dr);
+        
+        LET ret : Struct DivOutStr <- STRUCT { "quotient" ::= #q;
+                                               "remainder" ::= #rem
+                                             };
+        Ret #ret
+            
+      with Rule "divStep" :=
+        Read cnt : Bit DivLogNumPhases <- "cnt";
+        Assert (#cnt != $0);
+
+        Read pq : Bit (DivNumBits + S DivNumBits) <- "pq";
+        Read dr : Bit DivNumBits <- "dr";
+        
+        divSteps
+          DivNumBitsPerPhase pq dr
+          (fun npq => Write "pq" <- #npq; Retv)
+    }.
+
+  Definition dividerSpec :=
+    MODULE {
+      Register "quotient" : Bit DivNumBits <- Default
+      with Register "remainder" : Bit DivNumBits <- Default
+                         
+      with Method "divRegister"(src: Struct DivInStr): Void :=
+        LET m : Bit DivNumBits <- #src!DivInStr@."dividend";
+        LET r : Bit DivNumBits <- #src!DivInStr@."divisor";
+
+        Write "quotient" <- #m / #r;
+        Write "remainder" <- BinBit (Rem _ SignSS) #m #r;
+        Retv
+
+      with Method "divGetResult"(): Struct DivOutStr :=
+        Read quotient : Bit DivNumBits <- "quotient";
+        Read remainder : Bit DivNumBits <- "remainder";
+
+        LET ret : Struct DivOutStr <- STRUCT { "quotient" ::= #quotient;
+                                               "remainder" ::= #remainder };
+        Ret #ret
+    }.
+  
+End Divider64.
+
