Puar/Multiplier.v
@@ -1,0 +1,168 @@
+Require Import Kami.
+Require Import Lib.Indexer Lib.Struct Lib.FMap Lib.Reflection.
+Require Import Kami.Tactics Kami.SemFacts Kami.StepDet.
+Require Import Puar.Useful FunctionalExtensionality.
+
+Set Implicit Arguments.
+Open Scope string.
+(* Below implements a radix-4 Booth Multiplier.
+ *
+ * Note that the Booth multiplication algorithm is naturally designed
+ * for signed integers, so we need to add sign bits (0) for unsigned integers
+ * and their multiplication. It means we have to deal with 65 bits for 64-bit
+ * unsigned multiplication.
+ *
+ * Here we assume the multiplier always takes _65-bit signed integers_ as
+ * arguments.
+ *)
+Section Multiplier64.
+  (* NOTE: hard to declare [LogNumPhases] and [NumBitsPerPhase] as variables,
+   * since truncation and extension require certain equation w.r.t. bit-lengths.
+   *)
+  (* Variable MultLogNumPhases MultNumStepsPerPhase: nat. *)
+  Definition MultLogNumPhases := 3.
+  Definition MultNumStepsPerPhase := 4.
+  (* 2*4 = 8 bits are calculated per a phase. *)
+  Definition MultNumBitsPerPhase := 2 * MultNumStepsPerPhase. 
+
+  Definition MultNumPhases := wordToNat (wones MultLogNumPhases) + 1. (* 2^3 = 8 *)
+  Definition MultNumBits := MultNumPhases * MultNumBitsPerPhase + 1. (* 8*8 + 1 = 65 *)
+  Definition MultBits := 2 * MultNumBits + 2.
+
+  Definition MultInStr := STRUCT { "multiplicand" :: Bit MultNumBits;
+                                   "multiplier" :: Bit MultNumBits }.
+  Definition MultOutStr := STRUCT { "high" :: Bit MultNumBits;
+                                    "low" :: Bit MultNumBits }.
+
+  Definition multRegister := MethodSig "multRegister"(Struct MultInStr): Void.
+  Definition multGetResult := MethodSig "multGetResult"(Void): Struct MultOutStr.
+
+  Definition boothStep' {ty}
+             (m_pos m_neg: fullType ty (SyntaxKind (Bit MultBits)))
+             (p: Expr ty (SyntaxKind (Bit MultBits)))
+             (pr: Expr ty (SyntaxKind (Bit 2))) :=
+    (IF (pr == $$(WO~0~1)) then p + #m_pos
+     else IF (pr == $$(WO~1~0)) then p - #m_pos
+     else p)%kami_expr.
+
+  Definition boothStep {ty}
+             (m_pos m_neg: fullType ty (SyntaxKind (Bit MultBits)))
+             (p: Expr ty (SyntaxKind (Bit ((MultBits - 2) + 2))))
+    : Expr ty (SyntaxKind (Bit MultBits)) :=
+    (boothStep' m_pos m_neg p (UniBit (Trunc 2 _) p) >> $$(WO~1))%kami_expr.
+
+  Definition booth4Step' {ty}
+             (m_pos m_neg: fullType ty (SyntaxKind (Bit MultBits)))
+             (p: Expr ty (SyntaxKind (Bit MultBits)))
+             (pr: Expr ty (SyntaxKind (Bit 3))) :=
+    (IF (pr == $$(WO~0~0~1)) then p + #m_pos
+     else IF (pr == $$(WO~0~1~0)) then p + #m_pos
+     else IF (pr == $$(WO~0~1~1)) then p + (#m_pos << $$(WO~1))
+     else IF (pr == $$(WO~1~0~0)) then p + (#m_pos << $$(WO~1))
+     else IF (pr == $$(WO~1~0~1)) then p + #m_neg
+     else IF (pr == $$(WO~1~1~0)) then p + #m_neg
+     else p)%kami_expr.
+
+  Definition booth4Step {ty}
+             (m_pos m_neg: fullType ty (SyntaxKind (Bit MultBits)))
+             (p: Expr ty (SyntaxKind (Bit ((MultBits - 3) + 3))))
+    : Expr ty (SyntaxKind (Bit MultBits)) :=
+    (booth4Step' m_pos m_neg p (UniBit (Trunc 3 _) p) >> $$(WO~1~0))%kami_expr.
+
+  Fixpoint booth4Steps (cnt: nat)
+           {ty} (m_pos m_neg: fullType ty (SyntaxKind (Bit MultBits)))
+           (p: fullType ty (SyntaxKind (Bit ((MultBits - 3) + 3))))
+           (cont: fullType ty (SyntaxKind (Bit ((MultBits - 3) + 3))) ->
+                  ActionT ty Void)
+    : ActionT ty Void :=
+    match cnt with
+    | O => (cont p)%kami_action
+    | S n => (LET np <- booth4Step m_pos m_neg #p;
+              booth4Steps n m_pos m_neg np cont)%kami_action
+    end.
+
+  Definition boothMultRegister :=
+    MethodSig "boothMultRegister"(Struct MultInStr): Void.
+  Definition boothMultGetResult :=
+    MethodSig "boothMultGetResult"(): Struct MultOutStr.
+
+  Definition boothMultiplierImpl :=
+    MODULE {
+      Register "m_pos" : Bit MultBits <- Default
+      with Register "m_neg" : Bit MultBits <- Default
+      with Register "p" : Bit MultBits <- Default
+      with Register "cnt" : Bit (S MultLogNumPhases) <- Default
+
+      with Method "boothMultRegister"(src: Struct MultInStr): Void :=
+        LET m : Bit (pred MultNumBits + 1) <- #src!MultInStr@."multiplicand";
+        LET m_neg <- (UniBit (Inv _) #m) + $1;
+
+        LET m_pos : Bit MultBits <-
+          BinBit (Concat _ (S MultNumBits)) (UniBit (SignExtendTrunc _ _) #m) $0;
+        LET m_neg : Bit MultBits <-
+          BinBit (Concat _ (S MultNumBits)) (UniBit (SignExtendTrunc _ _) #m_neg) $0;
+        LET r <- #src!MultInStr@."multiplier";
+        LET p : Bit MultBits <-
+          BinBit (Concat (S MultNumBits) _) $0 (BinBit (Concat _ 1) #r $0);
+
+        (* Handle one bit in advance, in order to deal with other 64 bits 
+         * consistently in a rule [boothStep].
+         *)
+        LET np : Bit MultBits <- boothStep m_pos m_neg #p;
+        Write "m_pos" <- #m_pos;
+        Write "m_neg" <- #m_neg;
+        Write "p" <- #np;
+
+        Write "cnt" : Bit (S MultLogNumPhases) <- $(MultNumPhases);
+        Retv
+
+      with Method "boothMultGetResult"(): Struct MultOutStr :=
+        Read cnt : Bit MultLogNumPhases <- "cnt";
+        Assert (#cnt == $0);
+
+        Read p : Bit MultBits <- "p";
+        LET high : Bit MultNumBits <- UniBit (ConstExtract (S MultNumBits) MultNumBits 1) #p;
+        LET low : Bit MultNumBits <- UniBit (ConstExtract 1 MultNumBits (S MultNumBits)) #p;
+
+        LET ret : Struct MultOutStr <- STRUCT { "high" ::= $$Default; "low" ::= #low };
+        Ret #ret
+            
+      with Rule "boothStep" :=
+        Read cnt : Bit MultLogNumPhases <- "cnt";
+        Assert (#cnt != $0);
+
+        Read m_pos : Bit MultBits <- "m_pos";
+        Read m_neg : Bit MultBits <- "m_neg";
+        Read p : Bit MultBits <- "p";
+
+        Write "cnt" <- #cnt - $1;
+        
+        booth4Steps
+          MultNumStepsPerPhase m_pos m_neg p
+          (fun np => Write "p" <- #np; Retv)
+    }.
+
+  Definition multiplierSpec :=
+    MODULE {
+      Register "p" : Bit (2 * MultNumBits) <- Default
+
+      with Method "multRegister"(src: Struct MultInStr): Void :=
+        LET m : Bit MultNumBits <- #src!MultInStr@."multiplicand";
+        LET m_ext : Bit (2 * MultNumBits) <- UniBit (SignExtendTrunc _ _) #m;
+        LET r : Bit MultNumBits <- #src!MultInStr@."multiplier";
+        LET r_ext : Bit (2 * MultNumBits) <- UniBit (SignExtendTrunc _ _) #m;
+
+        Write "p" <- #m_ext *s #r_ext;
+        Retv
+
+      with Method "multGetResult"(): Struct MultOutStr :=
+        Read p : Bit (MultNumBits + MultNumBits) <- "p";
+        LET high : Bit MultNumBits <- UniBit (TruncLsb _ _) #p;
+        LET low : Bit MultNumBits <- UniBit (Trunc _ _) #p;
+
+        LET ret : Struct MultOutStr <- STRUCT { "high" ::= #high; "low" ::= #low };
+        Ret #ret
+    }.
+
+End Multiplier64.
+
